theories/PlutusIR.v
@@ -1,0 +1,309 @@
+Require Import Coq.Strings.String.
+Require Import Coq.Lists.List.
+Require Import Coq.Arith.PeanoNat.
+Require Import Coq.ZArith.BinInt.
+Require Import Coq.Bool.BoolEq.
+Require Import Ascii.
+Require Import Eqdep.
+
+From MetaCoq.TypedExtraction Require Import Util.
+From MetaCoq.TypedExtraction Require Import Utils.
+(* To use bytestring.string *)
+From MetaCoq.Template Require Import MCUtils.
+
+Require Import Coq.Program.Basics.
+
+Import ListNotations.
+
+
+
+(*
+  Simplification of the names in the AST
+
+  In the AST that we dump in the plutus compiler, variables are represented with the Name type, which is
+  a pair of String and Int, where the Int (newtyped as Unique) is used as a compiler detail for cheap name
+  comparisons (see Language.PlutusCore.Name.
+
+  We ignore these details and treat names (both terms and types) as strings. The definitions
+  below have the same types as the original AST constructors, but forget the structure and
+  map to a string.
+
+  This simplifies the representation and especially recognizing equal subterms (since
+  compiler passes may reassign unique numbers).
+
+  Possible future approach: it is preferable to have to complete AST including e.g.
+  Uniques, but prove that they do not matter for evaluation and then remove them from
+  AST
+
+*)
+
+(** Recursivity and strictness *)
+Inductive Recursivity := NonRec | Rec.
+
+Inductive Strictness := NonStrict | Strict.
+
+(** Universes *)
+Inductive DefaultUni : Type :=
+    | DefaultUniInteger    (* : DefaultUni Z (* Integer *) *)
+    | DefaultUniByteString (* : DefaultUni string (* BS.ByteString *)*)
+    | DefaultUniString     (* : DefaultUni string (* String *)*)
+    | DefaultUniChar       (* : DefaultUni ascii (* Char *)*)
+    | DefaultUniUnit       (* : DefaultUni unit (* () *)*)
+    | DefaultUniBool       (* : DefaultUni bool (* Bool *)*)
+    .
+
+(** Existentials as a datype *)
+Inductive some {f : DefaultUni -> Type} :=
+  Some : forall {u : DefaultUni}, f u -> some.
+Arguments some _ : clear implicits.
+
+(** Builtin types *)
+Inductive typeIn (u : DefaultUni) :=
+  TypeIn : typeIn u.
+Arguments typeIn _ : clear implicits.
+
+(** Constants *)
+Definition unitype (x : DefaultUni) : Type :=
+  match x with
+    | DefaultUniInteger    => Z
+    | DefaultUniByteString => string
+    | DefaultUniString     => string
+    | DefaultUniChar       => ascii
+    | DefaultUniUnit       => unit
+    | DefaultUniBool       => bool
+  end.
+
+Inductive valueOf (u : DefaultUni) :=
+  ValueOf : unitype u -> valueOf u.
+Arguments ValueOf _ _ : clear implicits.
+
+(** Built-in functions*)
+Inductive DefaultFun :=
+    | AddInteger
+    | SubtractInteger
+    | MultiplyInteger
+    | DivideInteger
+    | QuotientInteger
+    | RemainderInteger
+    | ModInteger
+    | LessThanInteger
+    | LessThanEqInteger
+    | GreaterThanInteger
+    | GreaterThanEqInteger
+    | EqInteger
+    | Concatenate
+    | TakeByteString
+    | DropByteString
+    | SHA2
+    | SHA3
+    | VerifySignature
+    | EqByteString
+    | LtByteString
+    | GtByteString
+    | IfThenElse
+    | CharToString
+    | Append
+    | Trace.
+
+
+
+Section AST_term.
+
+  (** kinds *)
+  Inductive kind :=
+    | kind_Base : kind
+    | kind_Arrow : kind -> kind -> kind.
+
+  (** types *)
+  Inductive ty :=
+    | ty_Var : string -> ty
+    | ty_Fun : ty -> ty -> ty
+    | ty_IFix : ty -> ty -> ty
+    | ty_Forall : string -> kind -> ty -> ty
+    | ty_Builtin : @some typeIn -> ty
+    | ty_Lam : string -> kind -> ty -> ty
+    | ty_App : ty -> ty -> ty.
+
+  (*
+    Simplification of attached values in the AST
+
+    In the Haskell AST, term is a functor and each constructor may have a field of the type parameter
+    `a`. Since this seems to be used only for storing intermediate compiler data, it is ignored here.
+    (this works because the dumping code is ignoring it)
+  *)
+
+  (** Declarations *)
+  Inductive vdecl := VarDecl : string -> ty -> vdecl.
+  Record tvdecl := tyVarDecl
+    { tvd_name : string
+    ; tvd_kind : kind
+    }.
+
+  (* Constructor string and arity, needed for Scott encoding *)
+  Inductive constr := Constructor : vdecl -> nat -> constr.
+  Inductive dtdecl := Datatype : tvdecl -> list tvdecl -> string -> list constr -> dtdecl.
+
+  (** terms and bindings *)
+  Inductive term :=
+    | Let      : Recursivity -> list binding -> term -> term
+    | Var      : string -> term
+    | TyAbs    : string -> kind -> term -> term
+    | LamAbs   : string -> ty -> term -> term
+    | Apply    : term -> term -> term
+    | Constant : @some valueOf -> term
+    | Builtin  : DefaultFun -> term
+    | TyInst   : term -> ty -> term
+    | Error    : ty -> term
+    | IWrap    : ty -> ty -> term -> term
+    | Unwrap   : term -> term
+
+  with binding :=
+    | TermBind : Strictness -> vdecl -> term -> binding
+    | typeBind : tvdecl -> ty -> binding
+    | DatatypeBind : dtdecl -> binding
+  .
+
+  (* Similar to mkLet in Plutus: for an empty list of bindings it is the identity, otherwise
+     it constructs a let with a non-empty list of bindings *)
+  Definition mk_let (r : Recursivity) (bs : list binding) (t : term) : term :=
+    match bs with
+      | [] => t
+      | _  => Let r bs t
+    end
+.
+
+  (** ** Trace of compilation *)
+  Inductive pass :=
+    | PassRestring
+    | PasstypeCheck
+    | PassInline : list string -> pass
+    | PassDeadCode
+    | PassThunkRec
+    | PassFloatterm
+    | PassLetNonStrict
+    | PassLettypes
+    | PassLetRec
+    | PassLetNonRec.
+
+  Inductive compilation_trace :=
+    | CompilationTrace : term -> list (pass * term) -> compilation_trace.
+
+  Definition constructorstring :=
+    fun c => match c with
+    | Constructor (VarDecl n _) _ => n
+    end
+    .
+
+End AST_term.
+
+
+Section term_rect.
+
+  Unset Implicit Arguments.
+
+  Variable (P : term -> Type).
+  Variable (Q : binding -> Type).
+
+  Context
+    (H_Let      : forall rec bs t, ForallT Q bs -> P t -> P (Let rec bs t))
+    (H_Var      : forall s : string, P (Var s))
+    (H_TyAbs    : forall (s : string) (k : kind) (t : term), P t -> P (TyAbs s k t))
+    (H_LamAbs   : forall (s : string) (t : ty) (t0 : term), P t0 -> P (LamAbs s t t0))
+    (H_Apply    : forall t : term, P t -> forall t0 : term, P t0 -> P (Apply t t0))
+    (H_Constant : forall s : some valueOf, P (Constant s))
+    (H_Builtin  : forall d : DefaultFun, P (Builtin d))
+    (H_TyInst   : forall t : term, P t -> forall t0 : ty, P (TyInst t t0))
+    (H_Error    : forall t : ty, P (Error t))
+    (H_IWrap    : forall (t t0 : ty) (t1 : term), P t1 -> P (IWrap t t0 t1))
+    (H_Unwrap   : forall t : term, P t -> P (Unwrap t)).
+
+  Context
+    (H_TermBind : forall s v t, P t -> Q (TermBind s v t))
+    (H_typeBind : forall v ty, Q (typeBind v ty))
+    (H_DatatypeBind : forall dtd, Q (DatatypeBind dtd)).
+
+  Definition bindings_rect' (binding_rect' : forall (b : binding), Q b) :=
+    fix bindings_rect' bs :=
+    match bs as p return ForallT Q p with
+      | nil       => ForallT_nil
+      | cons b bs => ForallT_cons (binding_rect' b) (bindings_rect' bs)
+    end.
+
+  Fixpoint term_rect' (t : term) : P t :=
+    match t with
+      | Let rec bs t    => H_Let rec bs t (bindings_rect' binding_rect' bs) (term_rect' t)
+      | Var n           => H_Var n
+      | TyAbs n k t     => H_TyAbs n k t (term_rect' t)
+      | LamAbs n ty t   => H_LamAbs n ty t (term_rect' t)
+      | Apply s t       => H_Apply s (term_rect' s) t (term_rect' t)
+      | TyInst t ty     => H_TyInst t (term_rect' t) ty
+      | IWrap ty1 ty2 t => H_IWrap ty1 ty2 t (term_rect' t)
+      | Unwrap t        => H_Unwrap t (term_rect' t)
+      | Error ty        => H_Error ty
+      | Constant v      => H_Constant v
+      | Builtin f       => H_Builtin f
+    end
+  with binding_rect' (b : binding) : Q b :=
+    match b with
+      | TermBind s v t  => H_TermBind s v t (term_rect' t)
+      | typeBind v ty   => H_typeBind v ty
+      | DatatypeBind dtd => H_DatatypeBind dtd
+    end.
+End term_rect.
+
+Section term__ind.
+
+  Unset Implicit Arguments.
+
+  Variable (P : term -> Prop).
+  Variable (Q : binding -> Prop).
+
+  Context
+    (H_Let      : forall rec bs t, ForallP Q bs -> P t -> P (Let rec bs t))
+    (H_Var      : forall s : string, P (Var s))
+    (H_TyAbs    : forall (s : string) (k : kind) (t : term), P t -> P (TyAbs s k t))
+    (H_LamAbs   : forall (s : string) (t : ty) (t0 : term), P t0 -> P (LamAbs s t t0))
+    (H_Apply    : forall t : term, P t -> forall t0 : term, P t0 -> P (Apply t t0))
+    (H_Constant : forall s : some valueOf, P (Constant s))
+    (H_Builtin  : forall d : DefaultFun, P (Builtin d))
+    (H_TyInst   : forall t : term, P t -> forall t0 : ty, P (TyInst t t0))
+    (H_Error    : forall t : ty, P (Error t))
+    (H_IWrap    : forall (t t0 : ty) (t1 : term), P t1 -> P (IWrap t t0 t1))
+    (H_Unwrap   : forall t : term, P t -> P (Unwrap t)).
+
+  Context
+    (H_TermBind : forall s v t, P t -> Q (TermBind s v t))
+    (H_typeBind : forall v ty, Q (typeBind v ty))
+    (H_DatatypeBind : forall dtd, Q (DatatypeBind dtd)).
+
+  Definition bindings__ind (binding__ind : forall (b : binding), Q b) :=
+    fix bindings__ind bs :=
+    match bs as p return ForallP Q p with
+      | nil       => ForallP_nil
+      | cons b bs => ForallP_cons (binding__ind b) (bindings__ind bs)
+    end.
+
+  Fixpoint term__ind (t : term) : P t :=
+    match t with
+      | Let rec bs t    => H_Let rec bs t (bindings__ind binding__ind bs) (term__ind t)
+      | Var n           => H_Var n
+      | TyAbs n k t     => H_TyAbs n k t (term__ind t)
+      | LamAbs n ty t   => H_LamAbs n ty t (term__ind t)
+      | Apply s t       => H_Apply s (term__ind s) t (term__ind t)
+      | TyInst t ty     => H_TyInst t (term__ind t) ty
+      | IWrap ty1 ty2 t => H_IWrap ty1 ty2 t (term__ind t)
+      | Unwrap t        => H_Unwrap t (term__ind t)
+      | Error ty        => H_Error ty
+      | Constant v      => H_Constant v
+      | Builtin f       => H_Builtin f
+    end
+  with binding__ind (b : binding) : Q b :=
+    match b with
+      | TermBind s v t  => H_TermBind s v t (term__ind t)
+      | typeBind v ty   => H_typeBind v ty
+      | DatatypeBind dtd => H_DatatypeBind dtd
+    end.
+
+  Combined Scheme term__multind from term__ind, binding__ind.
+
+End term__ind.
