theories/PlutusIR/Extract.v
@@ -1,0 +1,181 @@
+From MetaCoq.Template Require Import BasicAst utils.
+From MetaCoq.TypedExtraction Require Import ExAst.
+From MetaCoq.TypedExtraction Require Import PlutusIR.
+(* PlutusIR Erasure TypeAnnotations.*)
+From Coq Require Import Datatypes.
+From Coq Require Import Lists.List.
+
+Definition lift_a2 {A B C} : (A -> B -> C) -> option A -> option B -> option C :=
+  fun f x y => match x, y with
+  | Some v, Some w => Some (f v w)
+  | _, _ => None
+  end.
+
+Definition zip_with {A B C} (f : A -> B -> C) := 
+fix zip_with (l : list A) (l' : list B) {struct l} : list C :=
+  match l with
+  | [] => []
+  | x :: tl =>
+      match l' with
+      | [] => []
+      | y :: tl' => f x y :: zip_with tl tl'
+      end
+  end.
+
+(* TODO: generate actual fresh identifiers *)
+Definition print_name (n : name) : string :=
+  match n with
+  | nNamed s => s
+  | nAnon    => "_"
+  end.
+
+Module Types.
+
+  (* type variables *)
+  Definition trans (Δ : list tvdecl) : ExAst.box_type -> option PlutusIR.ty :=
+    fix trans bt :=
+      match bt with
+      | TArr τ τ' => lift_a2 ty_Fun (trans τ) (trans τ')
+      | TApp τ τ' => lift_a2 ty_App (trans τ) (trans τ')
+      | TVar i    => option_map (ty_Var ∘ tvd_name) (nth_error Δ i)
+      | TConst s  => Some (ty_Var (string_of_kername s))
+      | TInd ind  => Some (ty_Var (string_of_kername (inductive_mind ind)))
+      | TBox => Some (ty_Builtin (@PlutusIR.Some typeIn DefaultUniUnit (TypeIn DefaultUniUnit)))
+      | TAny => None
+      end.
+
+  (* Infer kinds of all free type variables, de Bruijn indexed *)
+  Axiom infer_kinds : box_type -> list kind.
+
+  Definition trans_ty_scheme (tyvars : list name) (τ : box_type) : option ty :=
+    let Δ : list tvdecl := zip_with tyVarDecl (map print_name tyvars) (infer_kinds τ) in
+    let add_foralls := fun τ_pir =>
+      fold_right (fun tvd σ => ty_Forall (tvd_name tvd) (tvd_kind tvd) σ) τ_pir Δ
+    in
+    option_map add_foralls (trans Δ τ)
+    .
+End Types.
+
+
+
+(* Some tests *)
+
+From MetaCoq.Template Require Import config Ast.
+From MetaCoq.TypedExtraction Require Import TypeAnnotations Erasure.
+From MetaCoq.PCUIC Require Import PCUICAst TemplateToPCUIC PCUICTyping.
+From MetaCoq.SafeChecker Require Import PCUICWfEnvImpl.
+
+Local Existing Instance fake_guard_impl_instance.
+Local Existing Instance extraction_checker_flags.
+Definition erase_type_impl (Σ : global_env_ext) (wfextΣ : ∥ wf_ext Σ∥) :=
+  @erase_type canonical_abstract_env_impl (ltac:(now unshelve econstructor;eauto)).
+
+Program Definition erase_type_program (p : Ast.Env.program) : global_env_ext * (list name * box_type) :=
+  let Σ := trans_global_env p.1 in
+  let Σext := empty_ext (PCUICProgram.trans_env_env Σ) in
+  (Σext, erase_type_impl Σext _ Σext eq_refl (trans Σ p.2) _).
+Next Obligation. Admitted.
+Next Obligation. Admitted.
+
+MetaCoq Quote Recursively Definition ex1 := (forall A, A -> A).
+Eval cbv in snd (erase_type_program ex1).
+Eval cbv in Types.trans
+  [tyVarDecl "A" kind_Base]
+  (TArr TBox (TArr (TVar 0) (TVar 0))).
+
+MetaCoq Quote Recursively Definition ex2:= (bool * bool -> bool).
+Definition ex2_erased_ty := snd (snd (erase_type_program ex2)).
+Eval cbv in Types.trans [] ex2_erased_ty.
+
+
+From MetaCoq.Erasure Require Import EAst.
+From MetaCoq.TypedExtraction Require Import Annotations.
+
+Module Terms.
+
+  Context (Δ : list tvdecl).
+  Fixpoint trans_mono
+    (Γ : list name) (* term vars *)
+    (t : term) : annots box_type t -> option PlutusIR.term :=
+    match t with
+
+    | tRel i => fun bt =>
+        Some (Var (print_name (nth i Γ nAnon)))
+
+    | tLambda na body => fun '(bt, a) =>
+        lift_a2 (LamAbs (print_name na)) (Types.trans Δ bt) (trans_mono (na :: Γ) body a)
+
+    | tApp hd arg => fun '(bt, (hda, arga)) =>
+        lift_a2 Apply (trans_mono Γ hd hda) (trans_mono Γ arg arga)
+
+    | _ => fun _ => None
+
+    end.
+
+  Definition trans
+    (t : EAst.term) (ann : annots box_type t) : option PlutusIR.term :=
+    let add_ty_abs := fun '(tyVarDecl v k) τ => TyAbs v k τ in
+    match trans_mono [] t ann with
+      | Some τ => Some (fold_right add_ty_abs τ Δ)
+      | None => None
+    end
+  .
+
+End Terms.
+
+Module Inductives.
+
+End Inductives.
+
+From MetaCoq.TypedExtraction Require Import Optimize.
+From MetaCoq.TypedExtraction Require Import Extraction.
+From MetaCoq.TypedExtraction Require Import ExAst.
+From MetaCoq.Template Require Import Ast.
+
+From MetaCoq.TypedExtraction Require Import ResultMonad.
+Import MCMonadNotation.
+
+
+(*
+   Needed for appropriate type inference of Monad below
+*)
+Definition result_bytestring_err A := result A bytestring.String.t.
+
+Definition to_lam_box (p : program) : result_bytestring_err _ :=
+  kn <- match p.2 with
+           | tConst kn _ => Ok kn
+           | tInd ind _ => Ok (inductive_mind ind)
+           | _ => Err ("Expected program to be a tConst or tInd")
+           end;;
+
+  Σ <- extract_template_env_within_coq
+         p.1
+         (KernameSet.singleton kn)
+         (fun k => false) ;;
+
+  ret Σ.
+
+From MetaCoq Require utils.
+
+Definition id (A : Set) (x : A) : A := x.
+
+MetaCoq Quote Recursively Definition t_id := id.
+Eval cbv in to_lam_box t_id.
+
+Definition to_lam_box_T (p : program) : result_bytestring_err (∑ Σ : ExAst.global_env, env_annots box_type Σ) :=
+  kn <- match p.2 with
+           | tConst kn _ => Ok kn
+           | tInd ind _ => Ok (inductive_mind ind)
+           | _ => Err ("Expected program to be a tConst or tInd")
+           end;;
+
+  match annot_extract_template_env_within_coq_sig
+         p.1
+         (KernameSet.singleton kn)
+         (fun k => false)
+  with
+  | None => Err "annot_extract_template_env_within_coq failed"
+  | Some (Σ ; env_anns) => Ok (Σ; env_anns)
+  end.
+
+Eval cbv in to_lam_box_T t_id.
